comment rename

Decompose_Update.thy
@@ -21,6 +21,7 @@ type_synonym 'y index = "'y \<times> nat"
 (* Shuffle *)
 type_synonym 'y shuffle = "'y \<Rightarrow> 'y list"
 
+(* unit operation of Shuffle *)
 definition idS :: "'y shuffle" where
   "idS \<equiv> (\<lambda>y. [y])"
 
@@ -41,48 +42,54 @@ fun scan_pair where
   "scan_pair x as (Inl y#u) = (x, as) # scan_pair y [] u" |
   "scan_pair x as (Inr a#u) = scan_pair x (as @ [a]) u"
 
-fun scan_head where
+fun scan_head :: "'b list \<Rightarrow> ('y + 'b) list \<Rightarrow> 'b list \<times> ('y \<times> 'b list) list" where
   "scan_head as [] = (as, [])" |
   "scan_head as (Inl x#u) = (as, scan_pair x [] u)" |
   "scan_head as (Inr a#u) = scan_head (as @ [a]) u"
 
-(* scan var-alphabet list, build pairs of a variable and a string *)
 definition scan :: "('y + 'b) list \<Rightarrow> 'b list \<times> ('y \<times> 'b list) list" where
   "scan u = scan_head [] u"
+
+
+subsubsection \<open>Flat\<close>
+
+text \<open>flatten pairs\<close>
 
 fun flat_rec where
   "flat_rec [] = []" |
   "flat_rec ((x, as)#xas) = Inl x # map Inr as @ flat_rec xas"
 
-
-(* flatten pairs *)
 definition flat where
   "flat = (\<lambda>(b0, xas). map Inr b0 @ flat_rec xas)"
+
+
+subsubsection \<open>Padding\<close>
+
+text \<open>replace strings with a special meta-variable\<close>
 
 fun padding_rec :: "nat \<Rightarrow> 'x \<Rightarrow> ('x \<times> 'b list) list \<Rightarrow> ('x + 'x index) list" where
   "padding_rec n y [] = []" |
   "padding_rec n y ((x, _)#xs) = Inl x # Inr (y, n) # padding_rec (Suc n) y xs"
 
-(* replace strings a special meta-variable *)
 definition padding :: "'y \<Rightarrow> 'b list \<times> ('y \<times> 'b list) list \<Rightarrow> ('y + 'y index) list" where
   "padding y = (\<lambda>(a0, xs). Inr (y, 0) # padding_rec 1 y xs)"
 
 
-fun ith_string where
-  "ith_string [] k = []" |
-  "ith_string ((x,as)#xas) 0 = as" |
-  "ith_string (_#xas) (Suc k) = ith_string xas k"
+subsubsection \<open>Others\<close>
 
+fun nth_string where
+  "nth_string [] k = []" |
+  "nth_string ((x,as)#xas) 0 = as" |
+  "nth_string (_#xas) (Suc k) = nth_string xas k"
 
-lemma ith_string_append_length: "ith_string (xs @ ys) (length xs) = ith_string ys 0"
+lemma nth_string_append_length: "nth_string (xs @ ys) (length xs) = nth_string ys 0"
   by (induct xs arbitrary: ys, simp_all)
-
 
 definition flat_store where
   "flat_store xs yi = (case yi of
     (Inl y) \<Rightarrow> [Inl y] |
     (Inr (x, 0)) \<Rightarrow> map Inr (fst xs) |
-    (Inr (x, Suc k)) \<Rightarrow> map Inr (ith_string (snd xs) k))"
+    (Inr (x, Suc k)) \<Rightarrow> map Inr (nth_string (snd xs) k))"
 
 lemma flat_rec_scan_pair: "flat_rec (scan_pair x as u) = Inl x # map Inr as @ u"
   by (induct u arbitrary: x as rule: xa_induct, simp_all)
@@ -92,18 +99,16 @@ lemma flat_scan_head: "flat (scan_head as u) = map Inr as @ u"
 
 lemma scan_inverse: "flat (scan u) = u"
 proof (induct u rule: xa_induct)
-  case Nil
-  then show ?case by (simp add: flat_def scan_def)
+  case Nil then show ?case by (simp add: flat_def scan_def)
 next
-  case (Var x xs)
-  then show ?case by (simp add: flat_def scan_def flat_rec_scan_pair)
+  case (Var x xs) then show ?case by (simp add: flat_def scan_def flat_rec_scan_pair)
 next
-  case (Alpha a xs)
-  then show ?case by (simp add: flat_scan_head scan_def)
+  case (Alpha a xs) then show ?case by (simp add: flat_scan_head scan_def)
 qed
 
 
 subsection \<open>Resolve\<close>
+text \<open>\<pi> in the thesis\<close>
 
 definition resolve_shuffle :: "('y, 'b) update \<Rightarrow> 'y shuffle" where
   "resolve_shuffle \<theta> y = extract_variables (\<theta> y)"
@@ -111,14 +116,14 @@ definition resolve_shuffle :: "('y, 'b) update \<Rightarrow> 'y shuffle" where
 definition resolve_store :: "('y, 'b) update \<Rightarrow> ('y, 'b) store" where
   "resolve_store \<theta> y = (case y of
      (x, 0) \<Rightarrow> fst (scan (\<theta> x)) |
-     (x, Suc k) \<Rightarrow> ith_string (snd (scan (\<theta> x))) k)"
+     (x, Suc k) \<Rightarrow> nth_string (snd (scan (\<theta> x))) k)"
 
-(* \<pi> *)
 fun resolve :: "('y, 'b) update \<Rightarrow> 'y shuffle \<times> ('y, 'b) store" where
   "resolve \<theta> = (resolve_shuffle \<theta>, resolve_store \<theta>)"
 
 
 subsection \<open>Synthesize\<close>
+text \<open>inverse of \<pi> in the thesis\<close>
 
 definition synthesize_shuffle :: "'y shuffle \<Rightarrow> ('y, 'y + 'y index, 'b) update'" where
   "synthesize_shuffle s y = map Inl (padding y (scan (map Inl (s y) :: ('y + 'y) list)))"
@@ -130,7 +135,6 @@ definition synthesize_store :: "('y, 'b) store \<Rightarrow> ('y + 'y index, 'y,
 
 fun synthesize :: "'y shuffle \<times> ('y, 'b) store \<Rightarrow> ('y, 'b) update" where
   "synthesize (s, a) = synthesize_store a \<bullet> synthesize_shuffle s"
-
 
 
 subsection \<open>Properties of Decomposition\<close>
@@ -269,7 +273,7 @@ next
   show ?case proof (cases xas)
     case (Pair x as)
     then show ?thesis
-      by (simp add: snoc, simp add: flat_store_def ith_string_append_length)
+      by (simp add: snoc, simp add: flat_store_def nth_string_append_length)
   qed
 qed
 
@@ -281,7 +285,7 @@ next
   case (snoc xas xs) then show ?case proof (cases xas)
     case (Pair y as)
     then show ?thesis apply (simp add: snoc flat_store_padding_append)
-      apply (simp add: flat_store_def ith_string_append_length)
+      apply (simp add: flat_store_def nth_string_append_length)
       done
   qed
 qed
